build-debug/out/lean/Lemmas.lean
@@ -15,16 +15,22 @@ set_option maxHeartbeats 10000000
 theorem correct___eo_prog_contra (M : SmtModel) (x1 x2 : Term) :
   (eo_interprets M x1 true) ->
   (eo_interprets M x2 true) ->
-  (Not (eo_interprets (__eo_prog_contra (Proof.pf x1) (Proof.pf x2)) false)) :=
+  (Not ((__eo_prog_contra (Proof.pf x1) (Proof.pf x2)) = Term.Stuck)) ->
+  (eo_interprets M (__eo_prog_contra (Proof.pf x1) (Proof.pf x2)) true) :=
 by
   sorry
 
 /- correctness theorem for __eo_prog_symm -/
 theorem correct___eo_prog_symm (M : SmtModel) (x1 : Term) :
   (eo_interprets M x1 true) ->
-  (Not (eo_interprets (__eo_prog_symm (Proof.pf x1)) false)) :=
+  (Not ((__eo_prog_symm (Proof.pf x1)) = Term.Stuck)) ->
+  (eo_interprets M (__eo_prog_symm (Proof.pf x1)) true) :=
 by
   sorry
 
+
+
+
+/- Helper definitions -/
 
 
