plugins/lean_meta/lean_meta_spec.lean
@@ -21,14 +21,14 @@ This is to be defined externally.
 -/
 abbrev ObjectTerm := SmtTerm
 
+abbrev ObjectModel := SmtModel
+
 /-
 A predicate defining a relation on terms in the object language and Booleans
 such that (s,b) is true if s evaluates to b.
 This is to be defined externally.
 -/
 abbrev obj_interprets := smt_interprets
-
-abbrev ObjectModel := SmtModel
 
 /-
 Definitions for eo_is_obj
